Checkpoint frontend FetchAndIncrement proof

src/program_proof/fencing/ctr_proof.v
@@ -10,69 +10,43 @@ Context `{!heapGS Σ}.
 Record ctr_names :=
   {}.
 
-Definition epoch_ptsto (e:u64) : iProp Σ.
+Definition own_epoch (e:u64) (q:Qp): iProp Σ.
 Admitted.
 
-Definition kv_epoch_ptsto (k e:u64) (v:option u64) : iProp Σ.
+Definition own_val (e:u64) (v:option u64) (q:Qp): iProp Σ.
 Admitted.
 
-Definition kv_ptsto (k v:u64) : iProp Σ.
+Global Instance own_epoch_timeless e q : Timeless (own_epoch e q).
+Admitted.
+
+Global Instance own_val_timeless e v q : Timeless (own_val e v q).
 Admitted.
 
 Definition own_Clerk (ck:loc) : iProp Σ.
 Admitted.
 
-
-(* |={Eo,Ei}=> ∃ vold, kv_ptsto k vold ∗ (kv_ptsto k vnew ={Ei,Eo}=∗ Q) *)
-
-(* XXX: the current Clerk is a sequential clerk: can only do one operation at a
-   time with it. Will need to have multiple CIDs to do multiple operations. *)
-
-Lemma wp_Clerk__Put_typical {Eo Ei:coPset} Φ (k v:u64):
-  (|={Eo,Ei}=> ∃ vold, kv_ptsto k vold ∗ (kv_ptsto k v ={Ei,Eo}=∗ Φ #v)) -∗
-    WP Clerk__Put #() @ Eo {{ Φ }}.
-Proof.
-Admitted.
-
-(*
-Lemma wp_Clerk__Put {Eo Ei:coPset} Φ (k e v:u64):
-  (|={Eo,Ei}=> ∃ vold, kv_ptsto k vold ∗ kv_epoch_ptsto k e vold ∗
-    (kv_ptsto k v ∗ kv_epoch_ptsto k e v ={Ei,Eo}=∗ Φ #v)) -∗
-    WP Clerk__Put #() @ Eo {{ Φ }}.
-Proof.
-Admitted.
-
-Lemma wp_Clerk__Put_unknown {Eo Ei:coPset} Φ (k e v:u64):
-  (|={Eo,Ei}=> ∃ vold, kv_ptsto k vold ∗ kv_epoch_unknown k e ∗
-    (kv_ptsto k v ∗ kv_epoch_ptsto k e v ={Ei,Eo}=∗ Φ #v)) -∗
-    WP Clerk__Put #() @ Eo {{ Φ }}.
-Proof.
-Admitted.
-*)
-
-Lemma wp_Clerk__Get {Eo Ei Ei2:coPset} ck (k e:u64) :
+Lemma wp_Clerk__Get {Eo Ei Ei2:coPset} ck (e:u64) :
   ∀ Φ,
   own_Clerk ck -∗
-  (|={Eo,Ei}=> ∃ latestEpoch, epoch_ptsto latestEpoch ∗
+  (|={Eo,Ei}=> ∃ latestEpoch, own_epoch latestEpoch (1/2)%Qp ∗
     (*(⌜int.Z latestEpoch > int.Z e⌝ → epoch_ptsto latestEpoch ={Ei, Eo}=∗ Φ #EStale) ∗*) (* XXX: program exits in this case *)
-    (⌜int.Z latestEpoch ≤ int.Z e⌝ → epoch_ptsto e ={Ei}=∗ (* XXX: one inner mask is probably enough, thhough we could have multiple invariants *)
-     (∃ oldv, kv_epoch_ptsto k e oldv ∗ (∃ v, ⌜is_Some oldv → oldv = Some v⌝ →
-                                               kv_epoch_ptsto k e (Some v) ={Ei2,Eo}=∗
+    (⌜int.Z latestEpoch ≤ int.Z e⌝ → own_epoch e (1/2)%Qp ={Ei}=∗ (* XXX: one inner mask is probably enough, thhough we could have multiple invariants *)
+     (∃ oldv, own_val e oldv (1/2)%Qp ∗ (∃ v, ⌜is_Some oldv → oldv = Some v⌝ →
+                                               own_val e (Some v) (1/2)%Qp ={Ei2,Eo}=∗
                                                               (own_Clerk ck -∗ Φ #v))))) -∗
     WP Clerk__Get #ck #e @ Eo {{ Φ }}.
 Proof.
 Admitted.
 
-(*
-Lemma wp_Server__Put {Eo Ei:coPset} Φ (k e v:u64) (s args:loc):
-  (|={Eo,Ei}=> ∃ vold, kv_ptsto k vold ∗ kv_ptsto_epoch k e vold ∗
-    (kv_ptsto k v ∗ kv_ptsto_epoch k e v ={Ei,Eo}=∗ Φ #v)) -∗
-    WP Server__Put #s #args @ Eo {{ Φ }}.
+Lemma wp_Clerk__Put {Eo Ei Ei2:coPset} ck (k e v:u64) :
+  ∀ Φ,
+  own_Clerk ck -∗
+  (|={Eo,Ei}=> ∃ latestEpoch, own_epoch latestEpoch (1/2)%Qp ∗
+    (*(⌜int.Z latestEpoch > int.Z e⌝ → epoch_ptsto latestEpoch ={Ei, Eo}=∗ Φ #EStale) ∗*) (* XXX: program exits in this case *)
+    (⌜int.Z latestEpoch ≤ int.Z e⌝ → own_epoch e (1/2)%Qp ={Ei}=∗ (* XXX: one inner mask is probably enough, thhough we could have multiple invariants *)
+     (∃ oldv, own_val e oldv (1/2)%Qp ∗ (own_val e (Some v) (1/2)%Qp ={Ei2,Eo}=∗ (own_Clerk ck -∗ Φ #v))))) -∗
+    WP Clerk__Get #ck #e @ Eo {{ Φ }}.
 Proof.
-  iIntros "Hpre".
-  wp_lam.
-  wp_pures.
-  (* wp_loadField. *)
-Admitted. *)
+Admitted.
 
 End ctr_definitions.
