src/program_proof/fencing/frontend_proof.v
@@ -2,17 +2,26 @@ From Perennial.program_proof Require Import grove_prelude.
 From Goose.github_com.mit_pdos.gokv.fencing Require Import frontend.
 From Perennial.program_proof Require Import grove_prelude.
 From Perennial.program_proof.memkv Require Export rpc_lib rpc_proof rpc_spec.
+From Perennial.program_proof.fencing Require Export ctr_proof.
 
 Section frontend_proof.
 
 Context `{!heapGS Σ}.
 
-Definition own_Server (s:loc) epoch : iProp Σ :=
-  ∃ ck1 ck2,
+Local Definition q2 := (1/2)%Qp.
+Local Definition q4 := (1/4)%Qp.
+
+Definition own_Server (s:loc) (epoch:u64) : iProp Σ :=
+  ∃ (ck1 ck2:loc),
   "#Hepoch" ∷ readonly (s ↦[frontend.Server :: "epoch"] #epoch) ∗
   "Hck1" ∷ s ↦[frontend.Server :: "ck1"] #ck1 ∗
   "Hck2" ∷ s ↦[frontend.Server :: "ck1"] #ck2 ∗
-  (* TODO: add ownership of clerks *)
+  "Hck1_own" ∷ own_Clerk ck1 ∗
+  "Hck2_own" ∷ own_Clerk ck2 ∗
+
+  "Hghost1" ∷ (∃ ov, own_val epoch ov q4) ∗
+  (* either have 1/2, or have 1/4 and have witness that latestEpoch >= epoch *)
+  (* TODO: add second value *)
   "_" ∷ True.
 
 Definition frontendN := nroot .@ "frontend".
@@ -23,9 +32,28 @@ Definition is_Server s : iProp Σ :=
   "HmuInv" ∷ is_lock frontendN mu (∃ epoch, own_Server s epoch)
 .
 
+Definition k0 := (U64 0).
+Definition k1 := (U64 1).
+
+Definition kv_ptsto (k v:u64) : iProp Σ.
+Admitted.
+
+Global Instance kv_ptsto_timeless k v : Timeless (kv_ptsto k v).
+Admitted.
+
+Definition frontend_inv_def: iProp Σ :=
+  ∃ (latestEpoch v:u64),
+  "HlatestEpoch" ∷ own_epoch latestEpoch q2 ∗
+  "Hval" ∷ own_val latestEpoch (Some v) q4 ∗
+  "Hkv" ∷ kv_ptsto k0 v.
+
+Definition frontend_inv : iProp Σ :=
+  inv frontendN (frontend_inv_def).
+
 Lemma wp_FetchAndIncrement (s:loc) (key:u64) :
   key = 0 ∨ key = 1 →
   is_Server s -∗
+  frontend_inv -∗
   {{{
         True
   }}}
@@ -35,7 +63,7 @@ Lemma wp_FetchAndIncrement (s:loc) (key:u64) :
   }}}.
 Proof.
   intros Hkey.
-  iIntros "#Hsrv !#" (Φ) "_ HΦ".
+  iIntros "#Hsrv #Hinv !#" (Φ) "_ HΦ".
   wp_lam.
   wp_pures.
   iNamed "Hsrv".
@@ -52,6 +80,15 @@ Proof.
   {
     wp_loadField.
     wp_loadField.
-    wp_apply (wp_Clerk__Get_unknown).
+    wp_apply (wp_Clerk__Get with "Hck2_own").
+    iInv "Hinv" as ">Hown" "Hclose".
+    iNamed "Hown".
+    iModIntro.
+    iExists _; iFrame.
+    iIntros "%Hfresh HlatestEpoch".
+    iModIntro.
+    admit.
   }
+Admitted.
+
 End frontend_proof.
